Remove SimLocalF

src/opt/ReorderRelFence.v
@@ -23,16 +23,390 @@ Require Import Progress.
 Require Import SimMemory.
 Require Import SimPromises.
 Require Import SimLocal.
-Require Import SimLocalF.
 Require Import Compatibility.
 Require Import SimThread.
 
+Require Import FulfillStep.
 Require Import ReorderStep.
 
 Require Import Syntax.
 Require Import Semantics.
 
 Set Implicit Arguments.
+
+
+Definition local_relfenced (lc:Local.t) :=
+  (Local.mk (TView.mk
+               (fun _ => lc.(Local.tview).(TView.cur))
+               lc.(Local.tview).(TView.cur)
+               lc.(Local.tview).(TView.acq))
+            lc.(Local.promises)).
+
+Lemma local_relfenced_wf
+      lc mem
+      (WF: Local.wf lc mem):
+  Local.wf (local_relfenced lc) mem.
+Proof.
+  inv WF. econs; ss; eauto.
+  - inv TVIEW_WF. econs; ss. refl.
+  - inv TVIEW_CLOSED. econs; ss.
+Qed.
+
+Lemma sim_local_promise_relfenced
+      pview
+      lc1_src mem1_src
+      lc1_tgt mem1_tgt
+      lc2_tgt mem2_tgt
+      loc from to val released kind
+      (STEP_TGT: Local.promise_step lc1_tgt mem1_tgt loc from to val released lc2_tgt mem2_tgt kind)
+      (LOCAL1: sim_local pview lc1_src (local_relfenced lc1_tgt))
+      (MEM1: sim_memory mem1_src mem1_tgt)
+      (WF1_SRC: Local.wf lc1_src mem1_src)
+      (WF1_TGT: Local.wf lc1_tgt mem1_tgt)
+      (MEM1_SRC: Memory.closed mem1_src)
+      (MEM1_TGT: Memory.closed mem1_tgt):
+  exists lc2_src mem2_src,
+    <<STEP_SRC: Local.promise_step lc1_src mem1_src loc from to val (SimPromises.none_if loc to pview released) lc2_src mem2_src (SimPromises.kind_transf loc to pview kind)>> /\
+    <<LOCAL2: sim_local pview lc2_src (local_relfenced lc2_tgt)>> /\
+    <<MEM2: sim_memory mem2_src mem2_tgt>>.
+Proof.
+  inv LOCAL1. inv STEP_TGT.
+  exploit SimPromises.promise; eauto.
+  { apply WF1_SRC. }
+  { apply WF1_TGT. }
+  i. des.
+  exploit sim_memory_closed_opt_view; eauto. i.
+  exploit Memory.promise_future; try apply PROMISE_SRC; eauto.
+  { apply WF1_SRC. }
+  { apply WF1_SRC. }
+  { unfold SimPromises.none_if. condtac; ss. }
+  i. des.
+  esplits; eauto.
+  - econs; eauto. unfold SimPromises.none_if. condtac; ss.
+  - econs; eauto.
+Qed.
+
+Lemma sim_local_read_relfenced
+      pview
+      lc1_src mem1_src
+      lc1_tgt mem1_tgt
+      lc2_tgt
+      loc ts val released_tgt ord_src ord_tgt
+      (STEP_TGT: Local.read_step lc1_tgt mem1_tgt loc ts val released_tgt ord_tgt lc2_tgt)
+      (LOCAL1: sim_local pview lc1_src (local_relfenced lc1_tgt))
+      (MEM1: sim_memory mem1_src mem1_tgt)
+      (WF1_SRC: Local.wf lc1_src mem1_src)
+      (WF1_TGT: Local.wf lc1_tgt mem1_tgt)
+      (MEM1_SRC: Memory.closed mem1_src)
+      (MEM1_TGT: Memory.closed mem1_tgt)
+      (ORD: Ordering.le ord_src ord_tgt):
+  exists released_src lc2_src,
+    <<REL: View.opt_le released_src released_tgt>> /\
+    <<STEP_SRC: Local.read_step lc1_src mem1_src loc ts val released_src ord_src lc2_src>> /\
+    <<LOCAL2: sim_local pview lc2_src (local_relfenced lc2_tgt)>>.
+Proof.
+  inv LOCAL1. inv STEP_TGT.
+  exploit sim_memory_get; try apply MEM1; eauto. i. des.
+  esplits; eauto.
+  - econs; eauto. eapply TViewFacts.readable_mon; eauto. apply TVIEW.
+  - econs; eauto. inv TVIEW. ss. econs; s.
+    + i. unfold LocFun.find. etrans; [by apply WF1_SRC|].
+      eauto using View.join_l.
+    + repeat apply View.join_le; ss.
+      * unfold View.singleton_ur_if. repeat condtac; viewtac.
+      * repeat condtac; viewtac.
+    + repeat apply View.join_le; ss.
+      * unfold View.singleton_ur_if. repeat condtac; viewtac.
+      * repeat condtac; viewtac.
+Qed.
+
+Lemma sim_local_fulfill_relfenced
+      pview
+      lc1_src sc1_src mem1_src
+      lc1_tgt sc1_tgt mem1_tgt
+      lc2_tgt sc2_tgt
+      loc from to val releasedm_src releasedm_tgt released ord_src ord_tgt
+      (RELM_LE: View.opt_le releasedm_src releasedm_tgt)
+      (RELM_WF: View.opt_wf releasedm_src)
+      (RELM_CLOSED: Memory.closed_opt_view releasedm_src mem1_src)
+      (WF_RELM_TGT: View.opt_wf releasedm_tgt)
+      (ORD: Ordering.le ord_src ord_tgt)
+      (PVIEW: (Ordering.le Ordering.acqrel ord_tgt /\ SimPromises.mem loc to pview = false) \/
+              Ordering.le ord_tgt Ordering.plain)
+      (STEP_TGT: fulfill_step lc1_tgt sc1_tgt loc from to val releasedm_tgt released ord_tgt lc2_tgt sc2_tgt)
+      (LOCAL1: sim_local pview lc1_src (local_relfenced lc1_tgt))
+      (SC1: TimeMap.le sc1_src sc1_tgt)
+      (MEM1: sim_memory mem1_src mem1_tgt)
+      (WF1_SRC: Local.wf lc1_src mem1_src)
+      (WF1_TGT: Local.wf lc1_tgt mem1_tgt)
+      (SC1_SRC: Memory.closed_timemap sc1_src mem1_src)
+      (SC1_TGT: Memory.closed_timemap sc1_tgt mem1_tgt)
+      (MEM1_SRC: Memory.closed mem1_src)
+      (MEM1_TGT: Memory.closed mem1_tgt):
+  exists lc2_src sc2_src,
+    <<STEP_SRC: fulfill_step lc1_src sc1_src loc from to val releasedm_src (SimPromises.none_if loc to pview released) ord_src lc2_src sc2_src>> /\
+    <<LOCAL2: sim_local (SimPromises.unset loc to pview) lc2_src (local_relfenced lc2_tgt)>> /\
+    <<SC2: TimeMap.le sc2_src sc2_tgt>>.
+Proof.
+  guardH PVIEW.
+  inv STEP_TGT.
+  assert (RELT_LE:
+   View.opt_le
+     (TView.write_released lc1_src.(Local.tview) sc1_src loc to releasedm_src ord_src)
+     (TView.write_released lc1_tgt.(Local.tview) sc2_tgt loc to releasedm_tgt ord_tgt)).
+  { unguardH PVIEW. des.
+    - unfold TView.write_released.
+      condtac; [|by econs].
+      condtac; cycle 1.
+      { by destruct ord_src, ord_tgt; inv PVIEW; inv COND0. }
+      econs. unfold TView.write_tview. s.
+      repeat (condtac; aggrtac); try by apply WF1_TGT.
+      + rewrite <- View.join_r. rewrite <- ? View.join_l. apply LOCAL1.
+      + rewrite <- View.join_r. rewrite <- ? View.join_l.
+        etrans; [|apply LOCAL1]. apply WF1_SRC.
+    - unfold TView.write_released. repeat (condtac; viewtac).
+  }
+  assert (RELT_WF:
+   View.opt_wf (TView.write_released lc1_src.(Local.tview) sc1_src loc to releasedm_src ord_src)).
+  { unfold TView.write_released. condtac; econs.
+    repeat (try condtac; viewtac; try apply WF1_SRC).
+  }
+  exploit SimPromises.remove; try exact REMOVE;
+    try exact MEM1; try apply LOCAL1; eauto.
+  { apply WF1_SRC. }
+  { apply WF1_TGT. }
+  { apply WF1_TGT. }
+  i. des. esplits.
+  - econs; eauto.
+    + unfold SimPromises.none_if. condtac.
+      * unguardH PVIEW. des; ss. unfold TView.write_released. condtac; [|refl].
+        destruct ord_src, ord_tgt; inv ORD; inv PVIEW; inv COND0.
+      * etrans; eauto.
+    + unfold SimPromises.none_if. condtac; viewtac.
+    + eapply TViewFacts.writable_mon; try exact WRITABLE; eauto. apply LOCAL1.
+  - econs; eauto. inv LOCAL1. inv TVIEW. ss. econs; s.
+    + i. rewrite LocFun.add_spec. condtac; ss.
+      { subst. unfold LocFun.find. condtac; apply View.join_le; viewtac.
+        etrans; eauto. refl.
+      }
+      unfold LocFun.find. etrans; [by apply WF1_SRC|].
+      eauto using View.join_l.
+    + apply View.join_le; viewtac.
+    + apply View.join_le; viewtac.
+  - ss.
+Qed.
+
+Lemma sim_local_promise_not_lower
+      pview
+      lc1_src
+      lc1_tgt mem1_tgt loc from to val released_tgt lc1 mem2_tgt kind
+      (LOCAL: sim_local pview lc1_src (local_relfenced lc1_tgt))
+      (STEP: Local.promise_step lc1_tgt mem1_tgt loc from to val released_tgt lc1 mem2_tgt kind)
+      (KIND: negb (Memory.op_kind_is_lower kind)):
+  SimPromises.mem loc to pview = false.
+Proof.
+  destruct (SimPromises.mem loc to pview) eqn:X; ss.
+  inv LOCAL. inv PROMISES. exploit PVIEW; eauto. i. des.
+  inv STEP. inv PROMISE; ss.
+  - exploit Memory.add_get0; try exact PROMISES; eauto. i. des. congr.
+  - exploit Memory.split_get0; try exact PROMISES; eauto. i. des. congr.
+Qed.
+
+Lemma sim_local_write_relfenced
+      pview
+      lc1_src sc1_src mem1_src
+      lc1_tgt sc1_tgt mem1_tgt
+      lc2_tgt sc2_tgt mem2_tgt
+      loc from to val releasedm_src releasedm_tgt released_tgt ord_src ord_tgt kind
+      (RELM_LE: View.opt_le releasedm_src releasedm_tgt)
+      (RELM_SRC_WF: View.opt_wf releasedm_src)
+      (RELM_SRC_CLOSED: Memory.closed_opt_view releasedm_src mem1_src)
+      (RELM_TGT_WF: View.opt_wf releasedm_tgt)
+      (RELM_TGT_CLOSED: Memory.closed_opt_view releasedm_tgt mem1_tgt)
+      (ORD: Ordering.le ord_src ord_tgt)
+      (ORD_TGT: Ordering.le ord_tgt Ordering.plain \/ Ordering.le Ordering.acqrel ord_tgt)
+      (STEP_TGT: Local.write_step lc1_tgt sc1_tgt mem1_tgt loc from to val releasedm_tgt released_tgt ord_tgt lc2_tgt sc2_tgt mem2_tgt kind)
+      (LOCAL1: sim_local pview lc1_src (local_relfenced lc1_tgt))
+      (SC1: TimeMap.le sc1_src sc1_tgt)
+      (MEM1: sim_memory mem1_src mem1_tgt)
+      (WF1_SRC: Local.wf lc1_src mem1_src)
+      (WF1_TGT: Local.wf lc1_tgt mem1_tgt)
+      (SC1_SRC: Memory.closed_timemap sc1_src mem1_src)
+      (SC1_TGT: Memory.closed_timemap sc1_tgt mem1_tgt)
+      (MEM1_SRC: Memory.closed mem1_src)
+      (MEM1_TGT: Memory.closed mem1_tgt):
+  exists released_src lc2_src sc2_src mem2_src,
+    <<STEP_SRC: Local.write_step lc1_src sc1_src mem1_src loc from to val releasedm_src released_src ord_src lc2_src sc2_src mem2_src (SimPromises.kind_transf loc to pview kind)>> /\
+    <<REL2: View.opt_le released_src released_tgt>> /\
+    <<LOCAL2: sim_local (SimPromises.unset loc to pview) lc2_src (local_relfenced lc2_tgt)>> /\
+    <<SC2: TimeMap.le sc2_src sc2_tgt>> /\
+    <<MEM2: sim_memory mem2_src mem2_tgt>>.
+Proof.
+  guardH ORD_TGT.
+  exploit write_promise_fulfill; eauto. i. des.
+  exploit Local.promise_step_future; eauto. i. des.
+  exploit sim_local_promise_relfenced; eauto. i. des.
+  exploit Local.promise_step_future; eauto. i. des.
+  assert (PVIEW: __guard__ ((Ordering.le Ordering.acqrel ord_tgt /\ SimPromises.mem loc to pview = false) \/
+                              Ordering.le ord_tgt Ordering.plain)).
+  { destruct (Ordering.le ord_tgt Ordering.strong_relaxed) eqn:X.
+    - right. unguardH ORD_TGT. destruct ord_tgt; des; ss.
+    - left. splits.
+      { by destruct ord_tgt; inv X. }
+      hexploit ORD0.
+      { by destruct ord_tgt; inv X. }
+      exploit Local.write_step_strong_relaxed; eauto.
+      { by destruct ord_tgt. }
+      i. eapply sim_local_promise_not_lower; try exact STEP1; eauto.
+  }
+  exploit sim_local_fulfill_relfenced; try apply STEP2;
+    try apply LOCAL2; try apply MEM2; eauto.
+  { eapply Memory.future_closed_opt_view; eauto. }
+  i. des.
+  exploit promise_fulfill_write; try exact STEP_SRC; try exact STEP_SRC0; eauto.
+  { i. hexploit ORD0; eauto.
+    i. des. subst. splits; auto. eapply sim_local_nonsynch_loc; eauto.
+  }
+  i. des. esplits; eauto.
+  - unguardH PVIEW. des.
+    + unfold SimPromises.none_if in *. rewrite PVIEW0 in *. ss.
+    + subst. unfold TView.write_released at 1. condtac; [|by econs].
+      destruct ord_src, ord_tgt; inv ORD; inv PVIEW; inv COND.
+  - etrans; eauto.
+Qed.
+
+Lemma sim_local_update_relfenced
+      pview
+      lc1_src sc1_src mem1_src
+      lc1_tgt sc1_tgt mem1_tgt
+      lc2_tgt
+      lc3_tgt sc3_tgt mem3_tgt
+      loc ts1 val1 released1_tgt ord1_src ord1_tgt
+      from2 to2 val2 released2_tgt ord2_src ord2_tgt kind
+      (STEP1_TGT: Local.read_step lc1_tgt mem1_tgt loc ts1 val1 released1_tgt ord1_tgt lc2_tgt)
+      (STEP2_TGT: Local.write_step lc2_tgt sc1_tgt mem1_tgt loc from2 to2 val2 released1_tgt released2_tgt ord2_tgt lc3_tgt sc3_tgt mem3_tgt kind)
+      (LOCAL1: sim_local pview lc1_src (local_relfenced lc1_tgt))
+      (SC1: TimeMap.le sc1_src sc1_tgt)
+      (MEM1: sim_memory mem1_src mem1_tgt)
+      (WF1_SRC: Local.wf lc1_src mem1_src)
+      (WF1_TGT: Local.wf lc1_tgt mem1_tgt)
+      (SC1_SRC: Memory.closed_timemap sc1_src mem1_src)
+      (SC1_TGT: Memory.closed_timemap sc1_tgt mem1_tgt)
+      (MEM1_SRC: Memory.closed mem1_src)
+      (MEM1_TGT: Memory.closed mem1_tgt)
+      (ORD1: Ordering.le ord1_src ord1_tgt)
+      (ORD2: Ordering.le ord2_src ord2_tgt)
+      (ORD2_TGT: Ordering.le ord2_tgt Ordering.plain \/ Ordering.le Ordering.acqrel ord2_tgt):
+  exists released1_src released2_src lc2_src lc3_src sc3_src mem3_src,
+    <<REL1: View.opt_le released1_src released1_tgt>> /\
+    <<REL2: View.opt_le released2_src released2_tgt>> /\
+    <<STEP1_SRC: Local.read_step lc1_src mem1_src loc ts1 val1 released1_src ord1_src lc2_src>> /\
+    <<STEP2_SRC: Local.write_step lc2_src sc1_src mem1_src loc from2 to2 val2 released1_src released2_src ord2_src lc3_src sc3_src mem3_src (SimPromises.kind_transf loc to2 pview kind)>> /\
+    <<LOCAL3: sim_local (SimPromises.unset loc to2 pview) lc3_src (local_relfenced lc3_tgt)>> /\
+    <<SC3: TimeMap.le sc3_src sc3_tgt>> /\
+    <<MEM3: sim_memory mem3_src mem3_tgt>>.
+Proof.
+  guardH ORD2_TGT.
+  exploit Local.read_step_future; eauto. i. des.
+  exploit sim_local_read_relfenced; eauto. i. des.
+  exploit Local.read_step_future; eauto. i. des.
+  hexploit sim_local_write_relfenced; eauto. i. des.
+  esplits; eauto.
+Qed.
+
+Lemma sim_local_fence_relfenced
+      pview
+      lc1_src sc1_src mem1_src
+      lc1_tgt sc1_tgt mem1_tgt
+      lc2_tgt sc2_tgt
+      ordr_src ordw_src
+      ordr_tgt ordw_tgt
+      (STEP_TGT: Local.fence_step lc1_tgt sc1_tgt ordr_tgt ordw_tgt lc2_tgt sc2_tgt)
+      (LOCAL1: sim_local pview lc1_src (local_relfenced lc1_tgt))
+      (SC1: TimeMap.le sc1_src sc1_tgt)
+      (MEM1: sim_memory mem1_src mem1_tgt)
+      (WF1_SRC: Local.wf lc1_src mem1_src)
+      (WF1_TGT: Local.wf lc1_tgt mem1_tgt)
+      (ORDR: Ordering.le ordr_src ordr_tgt)
+      (ORDW: Ordering.le ordw_src ordw_tgt)
+      (ORDR_TGT: Ordering.le ordr_tgt Ordering.acqrel)
+      (ORDW_TGT: Ordering.le ordw_tgt Ordering.relaxed):
+  exists lc2_src sc2_src,
+    <<STEP_SRC: Local.fence_step lc1_src sc1_src ordr_src ordw_src lc2_src sc2_src>> /\
+    <<LOCAL2: sim_local pview lc2_src (local_relfenced lc2_tgt)>> /\
+    <<SC2: TimeMap.le sc2_src sc2_tgt>>.
+Proof.
+  inv STEP_TGT. esplits; eauto.
+  - econs; eauto. i. eapply sim_local_nonsynch; eauto.
+  - inv LOCAL1. inv TVIEW. econs; ss.
+    econs; s; unfold LocFun.find; repeat condtac; aggrtac.
+    + etrans; eauto. apply WF1_TGT.
+    + etrans; eauto. apply WF1_TGT.
+    + etrans; eauto. apply WF1_TGT.
+  - unfold TView.write_fence_sc.
+    repeat (condtac; viewtac).
+Qed.
+
+Lemma sim_local_intro_relfenced
+      pview
+      lc1_src sc1_src mem1_src
+      lc1_tgt sc1_tgt mem1_tgt
+      (LOCAL1: sim_local pview lc1_src lc1_tgt)
+      (SC1: TimeMap.le sc1_src sc1_tgt)
+      (MEM1: sim_memory mem1_src mem1_tgt)
+      (WF1_SRC: Local.wf lc1_src mem1_src)
+      (WF1_TGT: Local.wf lc1_tgt mem1_tgt):
+  <<LOCAL2: sim_local pview lc1_src (local_relfenced lc1_tgt)>>.
+Proof.
+  esplits. inv LOCAL1. econs; eauto.
+  inv TVIEW. econs; ss; eauto.
+  etrans; eauto. apply WF1_TGT.
+Qed.
+
+Lemma sim_local_fence_src_relfenced
+      pview
+      lc1_src sc1_src mem1_src
+      lc1_tgt sc1_tgt mem1_tgt
+      (NONSYNCH: Memory.nonsynch lc1_src.(Local.promises))
+      (LOCAL1: sim_local pview lc1_src (local_relfenced lc1_tgt))
+      (SC1: TimeMap.le sc1_src sc1_tgt)
+      (MEM1: sim_memory mem1_src mem1_tgt)
+      (WF1_SRC: Local.wf lc1_src mem1_src)
+      (WF1_TGT: Local.wf lc1_tgt mem1_tgt):
+  exists lc2_src sc2_src,
+    <<STEP_SRC: Local.fence_step lc1_src sc1_src Ordering.plain Ordering.acqrel lc2_src sc2_src>> /\
+    <<LOCAL2: sim_local pview lc2_src (local_relfenced lc1_tgt)>> /\
+    <<SC2: TimeMap.le sc2_src sc1_tgt>>.
+Proof.
+  inv LOCAL1. inv TVIEW. ss.
+  esplits; eauto. econs; eauto. econs; ss; eauto.
+  repeat (condtac; aggrtac).
+Qed.
+
+Lemma sim_local_fence_tgt_relfenced
+      pview
+      lc1_src sc1_src mem1_src
+      lc1_tgt sc1_tgt mem1_tgt
+      lc2_tgt sc2_tgt
+      (STEP_TGT: Local.fence_step lc1_tgt sc1_tgt Ordering.plain Ordering.acqrel lc2_tgt sc2_tgt)
+      (LOCAL1: sim_local pview lc1_src (local_relfenced lc1_tgt))
+      (SC1: TimeMap.le sc1_src sc1_tgt)
+      (MEM1: sim_memory mem1_src mem1_tgt)
+      (WF1_SRC: Local.wf lc1_src mem1_src)
+      (WF1_TGT: Local.wf lc1_tgt mem1_tgt):
+  <<LOCAL2: sim_local SimPromises.bot lc1_src lc2_tgt>> /\
+  <<SC2: TimeMap.le sc1_src sc2_tgt>>.
+Proof.
+  inv LOCAL1. inv TVIEW. inv STEP_TGT. esplits; ss.
+  econs; s.
+  - unfold TView.read_fence_tview. condtac; ss.
+    unfold TView.write_fence_tview. econs; repeat (condtac; aggrtac).
+  - econs; try by apply PROMISES.
+    + inv PROMISES. ii. exploit LE; eauto.
+      unfold SimPromises.none_if. condtac; ss.
+      exploit RELEASE; eauto. s. i. subst. ss.
+    + i. rewrite SimPromises.bot_spec in *. congr.
+Qed.
 
 
 Inductive reorder_release_fenceF: forall (i2:Instr.t), Prop :=
@@ -58,7 +432,7 @@ Inductive sim_release_fenceF: forall (st_src:lang.(Language.state)) (lc_src:Loca
     pview
     lc1_src sc1_src mem1_src
     lc1_tgt sc1_tgt mem1_tgt
-    (LOCALF: sim_localF pview lc1_src lc1_tgt):
+    (LOCALF: sim_local pview lc1_src (local_relfenced lc1_tgt)):
     sim_release_fenceF
       (State.mk rs []) lc1_src sc1_src mem1_src
       (State.mk rs [Stmt.instr (Instr.fence Ordering.plain Ordering.acqrel)]) lc1_tgt sc1_tgt mem1_tgt
@@ -91,7 +465,7 @@ Proof.
   inv STEP_TGT; [inv STEP|inv STEP; inv LOCAL];
     try (inv STATE; inv INSTR); ss.
   - (* promise *)
-    exploit sim_localF_promise; eauto. i. des.
+    exploit sim_local_promise_relfenced; eauto. i. des.
     esplits.
     + eauto.
     + econs 2. econs 1. econs; eauto.
@@ -100,7 +474,7 @@ Proof.
     + auto.
     + right. econs 1; eauto.
   - (* fence *)
-    exploit sim_localF_elimination; try exact SC; eauto. i. des.
+    exploit sim_local_fence_tgt_relfenced; try exact SC; eauto. i. des.
     esplits.
     + eauto.
     + econs 1.
@@ -116,7 +490,7 @@ Proof.
   pcofix CIH. i. pfold. ii. ss. splits; ss.
   - i. inv TERMINAL_TGT. inv PR; ss.
   - i. inv PR.
-    exploit SimPromises.future; try apply LOCALF; eauto. i. des.
+    exploit SimPromises.future; (try by apply LOCALF); eauto using local_relfenced_wf. i. des.
     esplits.
     + etrans.
       { apply Memory.max_timemap_spec; eauto. viewtac. }
@@ -135,7 +509,7 @@ Proof.
     + auto.
   - i. inv PR.
     esplits; eauto.
-    eapply sim_localF_memory_bot; eauto.
+    eapply sim_local_memory_bot; eauto.
   - ii. exploit sim_release_fenceF_step; try apply PR; try apply SC; eauto. i. des.
     + esplits; eauto.
       left. eapply paco9_mon; eauto. ss.
@@ -171,14 +545,14 @@ Proof.
     esplits; try apply SC; eauto.
     - econs 2. econs 1; eauto. econs; eauto.
   }
-  exploit sim_localF_introduction; eauto. i. des.
-  exploit sim_localF_nonsynch_src; try exact SC_SRC; eauto. i. des.
+  exploit sim_local_intro_relfenced; eauto. i. des.
+  exploit sim_local_nonsynch_src; try exact SC_SRC; eauto using local_relfenced_wf. i. des.
   exploit Thread.rtc_tau_step_future; eauto. s. i. des.
-  exploit sim_localF_fence_src; eauto. i. des.
+  exploit sim_local_fence_src_relfenced; eauto. i. des.
   exploit Local.fence_step_future; eauto. i. des.
   inv STEP. inv LOCAL1; inv STATE; inv INSTR; inv REORDER.
   - (* load *)
-    exploit sim_localF_read; eauto; try refl. i. des.
+    exploit sim_local_read_relfenced; eauto; try refl. i. des.
     esplits.
     + etrans; [eauto|]. econs 2; [|refl]. econs.
       * econs. econs 2. econs; [|econs 5]; eauto. econs. econs.
@@ -191,7 +565,7 @@ Proof.
       econs. eauto.
   - (* update-load *)
     guardH ORDW2.
-    exploit sim_localF_read; eauto; try refl. i. des.
+    exploit sim_local_read_relfenced; eauto; try refl. i. des.
     esplits.
     + etrans; [eauto|]. econs 2; [|refl]. econs.
       * econs. econs 2. econs; [|econs 5]; eauto. econs. econs.
@@ -204,7 +578,7 @@ Proof.
       econs. eauto.
   - (* write *)
     guardH ORD2.
-    hexploit sim_localF_write; try exact SC; eauto;
+    hexploit sim_local_write_relfenced; try exact SC; eauto;
       (try refl); (try by econs). i. des.
     esplits.
     + etrans; [eauto|]. econs 2; [|refl]. econs.
@@ -220,9 +594,9 @@ Proof.
   - (* update *)
     guardH ORDW2.
     exploit Local.read_step_future; eauto. i. des.
-    exploit sim_localF_read; eauto; try refl. i. des.
+    exploit sim_local_read_relfenced; eauto; try refl. i. des.
     exploit Local.read_step_future; eauto. i. des.
-    hexploit sim_localF_write; try exact SC; eauto;
+    hexploit sim_local_write_relfenced; try exact SC; eauto;
       (try refl); (try by econs). i. des.
     esplits.
     + etrans; [eauto|]. econs 2; [|refl]. econs.
@@ -237,7 +611,7 @@ Proof.
     + left. eapply paco9_mon; [apply sim_release_fenceF_sim_thread|]; ss.
       econs. eauto.
   - (* fence *)
-    exploit sim_localF_fence; try exact SC; eauto; try refl. i. des.
+    exploit sim_local_fence_relfenced; try exact SC; eauto; try refl. i. des.
     esplits.
     + etrans; [eauto|]. econs 2; [|refl]. econs.
       * econs. econs 2. econs; [|econs 5]; eauto. econs. econs.
