src/opt/SimLocal.v
@@ -15,6 +15,7 @@ Require Import Language.
 Require Import View.
 Require Import Cell.
 Require Import Memory.
+Require Import MemoryFacts.
 Require Import TView.
 Require Import Local.
 Require Import Thread.
@@ -524,4 +525,122 @@ Proof.
     esplits; (try by econs; [|econs 5]; eauto); ss.
   - exploit sim_local_fence; eauto; try refl. i. des.
     esplits; (try by econs; [|econs 6]; eauto); ss.
+Qed.
+
+Lemma sim_local_lower_src
+      pview1
+      lc1_src sc1_src mem1_src
+      lc1_tgt mem1_tgt
+      lc2_src mem2_src
+      loc from to val released
+      (LOCAL1: sim_local pview1 lc1_src lc1_tgt)
+      (MEM1: sim_memory mem1_src mem1_tgt)
+      (WF1_SRC: Local.wf lc1_src mem1_src)
+      (WF1_TGT: Local.wf lc1_tgt mem1_tgt)
+      (SC1_SRC: Memory.closed_timemap sc1_src mem1_src)
+      (MEM1_SRC: Memory.closed mem1_src)
+      (STEP_SRC: Local.promise_step lc1_src mem1_src loc from to val None lc2_src mem2_src (Memory.op_kind_lower released)):
+  <<LOCAL2: exists pview2, sim_local pview2 lc2_src lc1_tgt>> /\
+  <<MEM2: sim_memory mem2_src mem1_tgt>> /\
+  <<WF2_SRC: Local.wf lc2_src mem2_src>>.
+Proof.
+  splits.
+  - inv STEP_SRC. inv PROMISE.
+    exists (match Memory.get loc to lc1_tgt.(Local.promises) with
+       | Some _ => SimPromises.set loc to pview1
+       | None => pview1
+       end).
+    inv LOCAL1. econs; ss. inv PROMISES0. econs; ss.
+    + ii.
+      exploit LE; eauto. i.
+      exploit Memory.lower_get0; try exact PROMISES; eauto. i.
+      erewrite Memory.lower_o; eauto.
+      unfold SimPromises.none_if.
+      destruct (Memory.get loc to (Local.promises lc1_tgt)) eqn:TGT.
+      * rewrite SimPromises.set_o. condtac; ss.
+        { des. subst. condtac; ss; cycle 1.
+          { revert COND0. condtac; ss. des; congr. }
+          rewrite GET in x. inv x. ss.
+        }
+        { guardH o. condtac.
+          { revert COND0. condtac; ss.
+            { des. subst. unguardH o. des; congr. }
+            guardH o0. i.
+            rewrite x. repeat f_equal. unfold SimPromises.none_if. condtac; ss.
+          }
+          rewrite x. repeat f_equal. unfold SimPromises.none_if. condtac; ss.
+          revert COND0. condtac; ss.
+        }
+      * condtac; ss. des. subst. congr.
+    + i. revert MEM0. condtac; ss; cycle 1.
+      { eapply PVIEW. }
+      rewrite SimPromises.set_o. condtac; ss; cycle 1.
+      { eapply PVIEW. }
+      i. des. subst. destruct p. eauto.
+    + i. revert SRC. erewrite Memory.lower_o; eauto. condtac; ss.
+      * i. des. inv SRC. eapply COMPLETE; eauto.
+        hexploit Memory.lower_get0; try exact PROMISES; eauto. i. des. eauto.
+      * i. eapply COMPLETE; eauto.
+  - etrans; [|eauto]. inv STEP_SRC. inv PROMISE. eapply lower_sim_memory. eauto.
+  - eapply Local.promise_step_future; eauto.
+Qed.
+
+Lemma sim_local_nonsynch_src
+      pview
+      lang st sc
+      lc1_src sc1_src mem1_src
+      lc1_tgt sc1_tgt mem1_tgt
+      (LOCAL1: sim_local pview lc1_src lc1_tgt)
+      (SC1: TimeMap.le sc1_src sc1_tgt)
+      (MEM1: sim_memory mem1_src mem1_tgt)
+      (LOCAL1_SRC: Local.wf lc1_src mem1_src)
+      (LOCAL2_TGT: Local.wf lc1_tgt mem1_tgt)
+      (SC1_SRC: Memory.closed_timemap sc1_src mem1_src)
+      (MEM1_SRC: Memory.closed mem1_src)
+      (MEM1_TGT: Memory.closed mem1_tgt):
+  exists pview2 lc2_src mem2_src,
+    <<STEP_SRC: rtc (@Thread.tau_step lang)
+                    (Thread.mk lang st lc1_src sc mem1_src)
+                    (Thread.mk lang st lc2_src sc mem2_src)>> /\
+    <<NONSYNCH2: Memory.nonsynch lc2_src.(Local.promises)>> /\
+    <<LOCAL2: sim_local pview2 lc2_src lc1_tgt>> /\
+    <<MEM2: sim_memory mem2_src mem1_tgt>>.
+Proof.
+  inversion LOCAL1_SRC. unfold Memory.finite in *. des.
+  assert (FINITE' : forall (loc : Loc.t) (from to : Time.t) (msg : Message.t),
+             Memory.get loc to (Local.promises lc1_src) =
+             Some (from, msg) -> msg.(Message.released) <> None -> In (loc, to) dom).
+  { ii. eapply FINITE. eauto. }
+  clear FINITE. move dom after lc1_src. revert_until dom. revert pview.
+  induction dom.
+  { esplits; eauto. ii. destruct (Message.released msg) eqn:X; ss.
+    exfalso. eapply FINITE'; eauto. congr.
+  }
+  destruct a as [loc to]. i.
+  destruct (Memory.get loc to lc1_src.(Local.promises)) as [[? []]|] eqn:X; cycle 1.
+  { eapply IHdom; eauto. i. exploit FINITE'; eauto. i. inv x; ss.
+    inv H1. congr.
+  }
+  destruct released; cycle 1.
+  { eapply IHdom; eauto. i. exploit FINITE'; eauto. i. inv x; ss.
+    inv H1. rewrite H in X. inv X. ss.
+  }
+  exploit MemoryFacts.promise_exists_None; eauto.
+  { eapply MemoryFacts.released_time_lt; [by apply MEM1_SRC|]. apply LOCAL1_SRC. eauto. }
+  i. des.
+  exploit Memory.promise_future; try apply LOCAL1_SRC; eauto; try by econs. i. des.
+  exploit sim_local_lower_src; eauto. i. des.
+  exploit IHdom; eauto.
+  { eapply Memory.future_closed_timemap; eauto. }
+  { eapply TView.future_closed; eauto. }
+  { s. i. inv x0. revert H.
+    erewrite Memory.lower_o; eauto. condtac; ss.
+    - i. des. inv H. ss.
+    - guardH o. i. exploit FINITE'; eauto. i. des; ss.  inv x.
+      unguardH o. des; congr.
+  }
+  i. des. esplits; try exact NONSYNCH2; eauto.
+  econs 2; eauto. econs.
+  - econs. econs 1. econs; eauto.
+  - ss.
 Qed.
